theories/examples_encoding_proofs.v
@@ -5,15 +5,15 @@ From osiris Require Import typing channel logrel.
 From iris.algebra Require Import list auth excl.
 From iris.base_logic Require Import invariants.
 From osiris Require Import encodable.
+From osiris Require Import examples.
 
 Section Encodings_Examples.
   Context `{!heapG Σ} {N : namespace}.
   Context `{!logrelG val Σ}.
 
-  Definition seq_example : expr :=
-    (let: "c" := new_chan #() in
-     send "c" #Left #5;;
-     recv "c" #Right)%E.
+  Notation "⟦ c @ s : sτ ⟧{ γ }" := (interp_st N γ (stype'_to_stype sτ) c s)
+    (at level 10, s at next level, sτ at next level, γ at next level,
+     format "⟦  c  @  s  :  sτ  ⟧{ γ }").
 
   Lemma seq_proof :
     {{{ True }}} seq_example {{{ v, RET v; ⌜v = #5⌝ }}}.
@@ -26,17 +26,11 @@ Section Encodings_Examples.
     wp_apply (send_st_enc_spec N Z with "[Hstl]")=> //. by iFrame.
     iIntros "Hstl".
     wp_apply (recv_st_enc_spec N Z with "[Hstr]"). iFrame.
-    iIntros (v w) "[Hstr [HP Heq]]".
+    iIntros (v) "[Hstr HP]".
     iApply "HΦ".
-    iDestruct "Heq" as %<-.
     iDestruct "HP" as %->.    
     eauto.
   Qed.
-
-  Definition par_2_example : expr :=
-    (let: "c" := new_chan #() in
-     Fork(let: "v" := recv "c" #Right in send "c" #Right ("v"+#4));;
-     send "c" #Left #5;;recv "c" #Left)%E.
 
   Lemma par_2_proof :
     {{{ True }}}
@@ -55,25 +49,18 @@ Section Encodings_Examples.
     wp_apply (wp_fork with "[Hstr]").
     - iNext.
       wp_apply (recv_st_enc_spec N Z with "[Hstr]"). by iFrame.
-      iIntros (v w) "[Hstr HP]".
-      iDestruct "HP" as %[HP <-].
+      iIntros (v) "[Hstr HP]".
       wp_apply (send_st_enc_spec N Z with "[Hstr]")=> //.
       iFrame; eauto 10 with iFrame.
-      iPureIntro. lia.
       eauto.
     - wp_apply (send_st_enc_spec N Z with "[Hstl]")=> //. by iFrame.
       iIntros "Hstl".
       wp_apply (recv_st_enc_spec N Z with "[Hstl]"). by iFrame.
-      iIntros (v w) "[Hstl HP]".
-      iDestruct "HP" as %[HP <-].
+      iIntros (v) "[Hstl HP]".
       iApply "HΦ".
+      iDestruct "HP" as %HP.
       iPureIntro. lia.
   Qed.
-
-  Definition heaplet_example : expr :=
-    (let: "c" := new_chan #() in
-     Fork(send "c" #Left (ref #5));;
-     !(recv "c" #Right))%E.
 
   Lemma heaplet_proof :
     {{{ True }}} heaplet_example {{{ v l, RET v; ⌜v = #5⌝ ∗ l ↦ v }}}.
@@ -91,26 +78,11 @@ Section Encodings_Examples.
       wp_apply (send_st_enc_spec N loc with "[Hstl HP]")=> //. by iFrame.
       eauto.
     - wp_apply (recv_st_enc_spec N loc with "[Hstr]"). iFrame.
-      iIntros (v w) "[Hstr HP]".
-      iDestruct "HP" as "[HP Henc]".
-      iDestruct "Henc" as %<-.
+      iIntros (v) "[Hstr HP]".
       wp_load.
       iApply "HΦ".
       iFrame. eauto.
   Qed.
-
-  Definition channel_example : expr :=
-    (let: "c" := new_chan #() in
-     Fork(
-         let: "c'" := new_chan #() in
-         send "c" #Left ("c'");; send "c'" #Left #5);;
-         let: "c'" := recv "c" #Right in
-         recv "c'" #Right
-    )%E.
-
-  Notation "⟦ c @ s : sτ ⟧{ γ }" := (interp_st N γ (stype'_to_stype sτ) c s)
-    (at level 10, s at next level, sτ at next level, γ at next level,
-     format "⟦  c  @  s  :  sτ  ⟧{ γ }").
 
   Lemma channel_proof :
     {{{ True }}} channel_example {{{ v, RET v; ⌜v = #5⌝ }}}.
@@ -136,12 +108,10 @@ Section Encodings_Examples.
       wp_apply (send_st_enc_spec N Z with "[Hstl']")=> //.
       iFrame. eauto. eauto.
     - wp_apply (recv_st_enc_spec N val with "[Hstr]")=> //.
-      iIntros (v w) "[Hstr [Hstr' Henc]]".
-      iDestruct "Henc" as %<-.
+      iIntros (v) "[Hstr Hstr']".
       iDestruct "Hstr'" as (γ') "Hstr'".
       wp_apply (recv_st_enc_spec N Z with "[Hstr']")=> //.
-      iIntros (v' w') "[Hstr' [HP Henc]]".
-      iDestruct "Henc" as %<-.
+      iIntros (v') "[Hstr' HP]".
       iDestruct "HP" as %<-.
       by iApply "HΦ".
   Qed.
