theories/examples.v
@@ -2,7 +2,6 @@ From iris.proofmode Require Import tactics.
 From iris.program_logic Require Export weakestpre.
 From iris.heap_lang Require Import proofmode notation.
 From osiris Require Import typing channel logrel.
-From iris.algebra Require Import list auth excl.
 From iris.base_logic Require Import invariants.
 
 Section Examples.
@@ -18,102 +17,20 @@ Section Examples.
      send "c" #Left #5;;
      recv "c" #Right)%E.
 
-  Lemma seq_proof :
-    {{{ True }}} seq_example {{{ v, RET v; ⌜v = #5⌝ }}}.
-  Proof.
-    iIntros (Φ H) "HΦ".
-    rewrite /seq_example.
-    wp_apply (new_chan_st_spec N (TSR Send (λ v, ⌜v = #5⌝%I) (λ v, TEnd)))=> //.
-    iIntros (c γ) "[Hstl Hstr]"=> /=.
-    wp_apply (send_st_spec N with "[$Hstl //]").
-    iIntros "Hstl".
-    wp_apply (recv_st_spec _ with "Hstr").
-    iIntros (v) "[Hstr HP]".
-    by iApply "HΦ".
-  Qed.
-
   Definition par_example : expr :=
     (let: "c" := new_chan #() in
      Fork(send "c" #Left #5);;
      recv "c" #Right)%E.
-
-  Lemma par_proof :
-    {{{ True }}} par_example {{{ v, RET v; ⌜v = #5⌝ }}}.
-  Proof.
-    iIntros (Φ H) "HΦ".
-    rewrite /par_example.
-    wp_apply (new_chan_st_spec N (TSR Send (λ v, ⌜v = #5⌝%I) (λ v, TEnd)))=> //.
-    iIntros (c γ) "[Hstl Hstr]"=> /=.
-    wp_apply (wp_fork with "[Hstl]").
-    - iNext. wp_apply (send_st_spec N with "[Hstl]"). by iFrame. eauto.
-    - wp_apply (recv_st_spec _ with "[Hstr]"). by iFrame.
-      iIntros (v) "[Hstr HP]". by iApply "HΦ".
-  Qed.
 
   Definition par_2_example : expr :=
     (let: "c" := new_chan #() in
      Fork(let: "v" := recv "c" #Right in send "c" #Right ("v"+#2));;
      send "c" #Left #5;;recv "c" #Left)%E.
 
-  Lemma par_2_proof :
-    {{{ True }}}
-      par_2_example
-    {{{ (v:Z), RET #v; ⌜7 ≤ v⌝ }}}.
-  Proof.
-    iIntros (Φ H) "HΦ".
-    rewrite /par_2_example.
-    wp_apply (new_chan_st_spec N
-      (TSR Send
-           (λ v, ⌜v = #5⌝%I)
-           (λ v, TSR Receive
-                     (λ v',
-                      (∃ w, ⌜v = LitV $ LitInt $ w⌝ ∧
-                       ∃ w', ⌜v' = LitV $ LitInt $ w' ∧ w' >= w+2⌝)%I)
-                     (λ v', TEnd))))=> //.
-    iIntros (c γ) "[Hstl Hstr]"=> /=.
-    wp_apply (wp_fork with "[Hstr]").
-    - iNext.
-      wp_apply (recv_st_spec _ with "[Hstr]"). by iFrame.
-      iIntros (v) "[Hstr HP]".
-      iDestruct "HP" as %->.
-      wp_apply (send_st_spec N with "[Hstr]"). iFrame; eauto 10 with iFrame.
-      eauto.
-    - wp_apply (send_st_spec _ with "[Hstl]"). by iFrame.
-      iIntros "Hstl".
-      wp_apply (recv_st_spec _ with "[Hstl]"). by iFrame.
-      iIntros (v) "[Hstl HP]".
-      iDestruct "HP" as %[w [HP [w' [-> HQ']]]].
-      iApply "HΦ".
-      iPureIntro. simplify_eq. lia.
-  Qed.
-
   Definition heaplet_example : expr :=
     (let: "c" := new_chan #() in
      Fork(send "c" #Left (ref #5));;
      !(recv "c" #Right))%E.
-
-  Lemma heaplet_proof :
-    {{{ True }}} heaplet_example {{{ v l, RET v; ⌜v = #5⌝ ∗ l ↦ v }}}.
-  Proof.
-    iIntros (Φ H) "HΦ".
-    rewrite /heaplet_example.
-    wp_apply (new_chan_st_spec N
-      (TSR Send (λ v, (∃ l, ⌜v = LitV $ LitLoc $ l⌝ ∧ (l ↦ #5))%I)
-                (λ v, TEnd)))=> //.
-    iIntros (c γ) "[Hstl Hstr]"=> /=.
-    wp_apply (wp_fork with "[Hstl]").
-    - iNext.
-      wp_apply (wp_alloc)=> //.
-      iIntros (l) "HP".
-      wp_apply (send_st_spec N with "[Hstl HP]"). eauto 10 with iFrame.
-      eauto.
-    - wp_apply (recv_st_spec _ with "[Hstr]"). by iFrame.
-      iIntros (v) "[Hstr HP]".
-      iDestruct "HP" as (l ->) "HP".
-      wp_load.
-      iApply "HΦ".
-      iFrame. eauto.
-  Qed.
 
   Definition channel_example : expr :=
     (let: "c" := new_chan #() in
@@ -124,75 +41,15 @@ Section Examples.
      recv "c'" #Right
     )%E.
 
-  Lemma channel_proof :
-    {{{ True }}} channel_example {{{ v, RET v; ⌜v = #5⌝ }}}.
-  Proof.
-    iIntros (Φ H) "HΦ".
-    rewrite /channel_example.
-    wp_apply (new_chan_st_spec N
-      (TSR Send (λ v, ∃ γ, ⟦ v @ Right :
-        (TSR Receive
-             (λ v : val, ⌜v = #5⌝)
-             (λ _ : val, TEnd)) ⟧{γ})%I
-                (λ v, TEnd)))=> //.
-    iIntros (c γ) "[Hstl Hstr]"=> /=.
-    wp_pures.
-    wp_apply (wp_fork with "[Hstl]").
-    - iNext.
-      wp_apply (new_chan_st_spec N
-        (TSR Send (λ v, ⌜v = #5⌝%I) (λ v, TEnd)))=> //.
-      iIntros (c' γ') "[Hstl' Hstr']"=> /=.
-      wp_apply (send_st_spec N with "[Hstl Hstr']").
-      iFrame. iExists γ'. iFrame.
-      iIntros "Hstl".
-      wp_apply (send_st_spec N with "[Hstl']").
-      iFrame. eauto. eauto.
-    - wp_apply (recv_st_spec _ with "[Hstr]"). by iFrame.
-      iIntros (v) "[Hstr Hstr']".
-      iDestruct "Hstr'" as (γ') "Hstr'".
-      wp_apply (recv_st_spec _ with "[Hstr']").
-      iApply "Hstr'".
-      iIntros (v') "[Hstr' HP]".
-      by iApply "HΦ".
-  Qed.
-
   Definition bad_seq_example : expr :=
     (let: "c" := new_chan #() in
      let: "v" := recv "c" #Right in
      send "c" #Left #5;; "v")%E.
 
-  Lemma bad_seq_proof :
-    {{{ True }}} bad_seq_example {{{ v, RET v; ⌜v = #5⌝ }}}.
-  Proof.
-    iIntros (Φ H) "HΦ".
-    rewrite /bad_seq_example.
-    wp_apply (new_chan_st_spec N (TSR Send (λ v, ⌜v = #5⌝%I) (λ v, TEnd)))=> //.
-    iIntros (c γ) "[Hstl Hstr]"=> /=.
-    wp_apply (recv_st_spec _ with "Hstr").
-    iIntros (v) "[Hstr HP]".
-    wp_apply (send_st_spec N with "[Hstl]"). by iFrame.
-    iIntros "Hstl".
-    wp_pures.
-    by iApply "HΦ".
-  Qed.
-
   Definition bad_par_example : expr :=
     (let: "c" := new_chan #() in
      Fork(#());;
      recv "c" #Right)%E.
-
-  Lemma bad_par_proof :
-    {{{ True }}} bad_par_example {{{ v, RET v; ⌜v = #5⌝ }}}.
-  Proof.
-    iIntros (Φ H) "HΦ".
-    rewrite /bad_par_example.
-    wp_apply (new_chan_st_spec N (TSR Send (λ v, ⌜v = #5⌝%I) (λ v, TEnd)))=> //.
-    iIntros (c γ) "[Hstl Hstr]"=> /=.
-    wp_apply (wp_fork with "[Hstl]").
-    - iNext. wp_finish. eauto.
-    - wp_apply (recv_st_spec _ with "[Hstr]"). by iFrame.
-      iIntros (v) "[Hstr HP]". by iApply "HΦ".
-  Qed.
 
   Definition bad_interleave_example : expr :=
     (let: "c" := new_chan #() in
@@ -200,25 +57,4 @@ Section Examples.
      Fork(recv "c" #Right;; send "c'" #Right #5);;
      recv "c'" #Left;; send "c" #Left #5)%E.
 
-  Lemma bad_interleave_proof :
-    {{{ True }}} bad_interleave_example {{{ v, RET v; ⌜v = #()⌝ }}}.
-  Proof.
-    iIntros (Φ H) "HΦ".
-    rewrite /bad_interleave_example.
-    wp_apply (new_chan_st_spec N (TSR Send (λ v, ⌜v = #5⌝%I) (λ v, TEnd)))=> //.
-    iIntros (c γ) "[Hstl Hstr]"=> /=.
-    wp_apply (new_chan_st_spec N (TSR Receive (λ v, ⌜v = #5⌝%I) (λ v, TEnd)))=> //.
-    iIntros (c' γ') "[Hstl' Hstr']"=> /=.
-    wp_apply (wp_fork with "[Hstr Hstr']").
-    - iNext. wp_apply (recv_st_spec _ with "[Hstr]"). by iFrame.
-      iIntros (v) "[Hstr HP]".
-      wp_apply (send_st_spec _ with "[Hstr']"). iFrame. eauto.
-      eauto.
-    - wp_apply (recv_st_spec _ with "[Hstl']"). by iFrame.
-      iIntros (v) "[Hstl' HP]".
-      wp_apply (send_st_spec _ with "[Hstl]"). iFrame. eauto.
-      iIntros "Hstl".
-      by iApply "HΦ".
-  Qed.
-  
 End Examples.
