theories/examples_proofs.v
@@ -1,0 +1,182 @@
+From iris.proofmode Require Import tactics.
+From iris.program_logic Require Export weakestpre.
+From iris.heap_lang Require Import proofmode notation.
+From osiris Require Import typing channel logrel.
+From iris.base_logic Require Import invariants.
+From osiris Require Import examples.
+
+Section ExampleProofs.
+  Context `{!heapG Σ} (N : namespace).
+  Context `{!logrelG val Σ}.
+
+  Notation "⟦ c @ s : sτ ⟧{ γ }" := (interp_st N γ sτ c s)
+    (at level 10, s at next level, sτ at next level, γ at next level,
+     format "⟦  c  @  s  :  sτ  ⟧{ γ }").
+
+  Lemma seq_proof :
+    {{{ True }}} seq_example {{{ v, RET v; ⌜v = #5⌝ }}}.
+  Proof.
+    iIntros (Φ H) "HΦ".
+    rewrite /seq_example.
+    wp_apply (new_chan_st_spec N (TSR Send (λ v, ⌜v = #5⌝%I) (λ v, TEnd)))=> //.
+    iIntros (c γ) "[Hstl Hstr]"=> /=.
+    wp_apply (send_st_spec N with "[$Hstl //]").
+    iIntros "Hstl".
+    wp_apply (recv_st_spec _ with "Hstr").
+    iIntros (v) "[Hstr HP]".
+    by iApply "HΦ".
+  Qed.
+
+  Lemma par_proof :
+    {{{ True }}} par_example {{{ v, RET v; ⌜v = #5⌝ }}}.
+  Proof.
+    iIntros (Φ H) "HΦ".
+    rewrite /par_example.
+    wp_apply (new_chan_st_spec N (TSR Send (λ v, ⌜v = #5⌝%I) (λ v, TEnd)))=> //.
+    iIntros (c γ) "[Hstl Hstr]"=> /=.
+    wp_apply (wp_fork with "[Hstl]").
+    - iNext. wp_apply (send_st_spec N with "[Hstl]"). by iFrame. eauto.
+    - wp_apply (recv_st_spec _ with "[Hstr]"). by iFrame.
+      iIntros (v) "[Hstr HP]". by iApply "HΦ".
+  Qed.
+
+  Lemma par_2_proof :
+    {{{ True }}}
+      par_2_example
+    {{{ (v:Z), RET #v; ⌜7 ≤ v⌝ }}}.
+  Proof.
+    iIntros (Φ H) "HΦ".
+    rewrite /par_2_example.
+    wp_apply (new_chan_st_spec N
+      (TSR Send
+           (λ v, ⌜v = #5⌝%I)
+           (λ v, TSR Receive
+                     (λ v',
+                      (∃ w, ⌜v = LitV $ LitInt $ w⌝ ∧
+                       ∃ w', ⌜v' = LitV $ LitInt $ w' ∧ w' >= w+2⌝)%I)
+                     (λ v', TEnd))))=> //.
+    iIntros (c γ) "[Hstl Hstr]"=> /=.
+    wp_apply (wp_fork with "[Hstr]").
+    - iNext.
+      wp_apply (recv_st_spec _ with "[Hstr]"). by iFrame.
+      iIntros (v) "[Hstr HP]".
+      iDestruct "HP" as %->.
+      wp_apply (send_st_spec N with "[Hstr]"). iFrame; eauto 10 with iFrame.
+      eauto.
+    - wp_apply (send_st_spec _ with "[Hstl]"). by iFrame.
+      iIntros "Hstl".
+      wp_apply (recv_st_spec _ with "[Hstl]"). by iFrame.
+      iIntros (v) "[Hstl HP]".
+      iDestruct "HP" as %[w [HP [w' [-> HQ']]]].
+      iApply "HΦ".
+      iPureIntro. simplify_eq. lia.
+  Qed.
+
+  Lemma heaplet_proof :
+    {{{ True }}} heaplet_example {{{ v l, RET v; ⌜v = #5⌝ ∗ l ↦ v }}}.
+  Proof.
+    iIntros (Φ H) "HΦ".
+    rewrite /heaplet_example.
+    wp_apply (new_chan_st_spec N
+      (TSR Send (λ v, (∃ l, ⌜v = LitV $ LitLoc $ l⌝ ∧ (l ↦ #5))%I)
+                (λ v, TEnd)))=> //.
+    iIntros (c γ) "[Hstl Hstr]"=> /=.
+    wp_apply (wp_fork with "[Hstl]").
+    - iNext.
+      wp_apply (wp_alloc)=> //.
+      iIntros (l) "HP".
+      wp_apply (send_st_spec N with "[Hstl HP]"). eauto 10 with iFrame.
+      eauto.
+    - wp_apply (recv_st_spec _ with "[Hstr]"). by iFrame.
+      iIntros (v) "[Hstr HP]".
+      iDestruct "HP" as (l ->) "HP".
+      wp_load.
+      iApply "HΦ".
+      iFrame. eauto.
+  Qed.
+
+  Lemma channel_proof :
+    {{{ True }}} channel_example {{{ v, RET v; ⌜v = #5⌝ }}}.
+  Proof.
+    iIntros (Φ H) "HΦ".
+    rewrite /channel_example.
+    wp_apply (new_chan_st_spec N
+      (TSR Send (λ v, ∃ γ, ⟦ v @ Right :
+        (TSR Receive
+             (λ v : val, ⌜v = #5⌝)
+             (λ _ : val, TEnd)) ⟧{γ})%I
+                (λ v, TEnd)))=> //.
+    iIntros (c γ) "[Hstl Hstr]"=> /=.
+    wp_pures.
+    wp_apply (wp_fork with "[Hstl]").
+    - iNext.
+      wp_apply (new_chan_st_spec N
+        (TSR Send (λ v, ⌜v = #5⌝%I) (λ v, TEnd)))=> //.
+      iIntros (c' γ') "[Hstl' Hstr']"=> /=.
+      wp_apply (send_st_spec N with "[Hstl Hstr']").
+      iFrame. iExists γ'. iFrame.
+      iIntros "Hstl".
+      wp_apply (send_st_spec N with "[Hstl']").
+      iFrame. eauto. eauto.
+    - wp_apply (recv_st_spec _ with "[Hstr]"). by iFrame.
+      iIntros (v) "[Hstr Hstr']".
+      iDestruct "Hstr'" as (γ') "Hstr'".
+      wp_apply (recv_st_spec _ with "[Hstr']").
+      iApply "Hstr'".
+      iIntros (v') "[Hstr' HP]".
+      by iApply "HΦ".
+  Qed.
+
+  Lemma bad_seq_proof :
+    {{{ True }}} bad_seq_example {{{ v, RET v; ⌜v = #5⌝ }}}.
+  Proof.
+    iIntros (Φ H) "HΦ".
+    rewrite /bad_seq_example.
+    wp_apply (new_chan_st_spec N
+               (TSR Send (λ v, ⌜v = #5⌝%I) (λ v, TEnd)))=> //.
+    iIntros (c γ) "[Hstl Hstr]"=> /=.
+    wp_apply (recv_st_spec _ with "Hstr").
+    iIntros (v) "[Hstr HP]".
+    wp_apply (send_st_spec N with "[Hstl]"). by iFrame.
+    iIntros "Hstl".
+    wp_pures.
+    by iApply "HΦ".
+  Qed.
+
+  Lemma bad_par_proof :
+    {{{ True }}} bad_par_example {{{ v, RET v; ⌜v = #5⌝ }}}.
+  Proof.
+    iIntros (Φ H) "HΦ".
+    rewrite /bad_par_example.
+    wp_apply (new_chan_st_spec N
+               (TSR Send (λ v, ⌜v = #5⌝%I) (λ v, TEnd)))=> //.
+    iIntros (c γ) "[Hstl Hstr]"=> /=.
+    wp_apply (wp_fork with "[Hstl]").
+    - iNext. wp_finish. eauto.
+    - wp_apply (recv_st_spec _ with "[Hstr]"). by iFrame.
+      iIntros (v) "[Hstr HP]". by iApply "HΦ".
+  Qed.
+
+  Lemma bad_interleave_proof :
+    {{{ True }}} bad_interleave_example {{{ v, RET v; ⌜v = #()⌝ }}}.
+  Proof.
+    iIntros (Φ H) "HΦ".
+    rewrite /bad_interleave_example.
+    wp_apply (new_chan_st_spec N (TSR Send (λ v, ⌜v = #5⌝%I) (λ v, TEnd)))=> //.
+    iIntros (c γ) "[Hstl Hstr]"=> /=.
+    wp_apply (new_chan_st_spec N
+               (TSR Receive (λ v, ⌜v = #5⌝%I) (λ v, TEnd)))=> //.
+    iIntros (c' γ') "[Hstl' Hstr']"=> /=.
+    wp_apply (wp_fork with "[Hstr Hstr']").
+    - iNext. wp_apply (recv_st_spec _ with "[Hstr]"). by iFrame.
+      iIntros (v) "[Hstr HP]".
+      wp_apply (send_st_spec _ with "[Hstr']"). iFrame. eauto.
+      eauto.
+    - wp_apply (recv_st_spec _ with "[Hstl']"). by iFrame.
+      iIntros (v) "[Hstl' HP]".
+      wp_apply (send_st_spec _ with "[Hstl]"). iFrame. eauto.
+      iIntros "Hstl".
+      by iApply "HΦ".
+  Qed.
+
+End ExampleProofs.
